FOL_completeness/GenCompleteness.v
@@ -1,0 +1,352 @@
+Require Export GenConstructions Consistency FOL_completeness.Tarski.
+(*From Undecidability.FOLC Require Import Stability.*)
+
+(** ** Completeness *)
+
+(* ** Standard Models **)
+
+Section Completeness.
+  Context {Σf : funcs_signature} {Σp : preds_signature}.
+  Context {HdF : eq_dec Σf} {HdP : eq_dec Σp}.
+  Context {HeF : enumerable__T Σf} {HeP : enumerable__T Σp}.
+
+  Hypothesis form_enum : nat -> form falsity_on.
+  Hypothesis form_enum_enumerates : forall phi, exists n : nat, form_enum n = phi.
+  Hypothesis form_enum_fresh : forall n m, n <= m -> unused m (form_enum n).
+
+  Hint Constructors unused.
+  Existing Instance falsity_on. 
+
+  Section BotModel.
+
+    Variable T : theory.
+    Hypothesis T_closed : closed_T T.
+
+    Definition input_bot :=
+      {|
+        NBot := falsity ;
+        NBot_closed := (fun n => uf_Fal n) ;
+
+        In_T := T ;
+        In_T_closed := T_closed ;
+
+        GenConstructions.enum := form_enum ;
+        GenConstructions.enum_enum := form_enum_enumerates ;
+        GenConstructions.enum_unused := form_enum_fresh
+      |}.
+
+    Definition output_bot := construct_construction input_bot.
+
+    Instance model_bot : interp term :=
+      {| i_func := func ; i_atom := fun P v => atom P v ∈ Out_T output_bot |}.
+
+    Lemma eval_ident rho (t : term) :
+      eval rho t = subst_term rho t.
+    Proof.
+      induction t using strong_term_ind; comp; try congruence. f_equal.
+    Qed.
+
+    Lemma form_ind_falsity (P : form falsity_on -> Prop) :
+      P ⊥ ->
+      (forall  (P0 : Σp) (t : t term (ar_preds P0)), P (atom P0 t)) ->
+      (forall  (b0 : binop) (f1 : form), P f1 -> forall f2 : form, P f2 -> P (bin b0 f1 f2)) ->
+      (forall (q : quantop) (f2 : form), P f2 -> P (quant q f2)) ->
+      forall (f4 : form), P f4.
+    Proof.
+    Admitted.
+
+    Lemma help phi t sigma :
+      phi[up sigma][t..] = phi[t.:sigma].
+    Proof.
+      rewrite subst_comp. apply subst_ext. intros [|]; cbn; trivial. unfold funcomp.
+      rewrite subst_term_comp. apply subst_term_id. now intros [].
+    Qed.
+
+    Hypothesis Hcon : consistent T.
+
+    Lemma model_bot_correct {ff : falsity_flag} phi rho :
+      (phi[rho] ∈ Out_T output_bot <-> rho ⊨ phi).
+    Proof.
+      revert rho. induction phi using form_ind_falsity; intros rho. 1,2,3: comp.
+      - split; try tauto. intros H. apply Hcon.
+        apply Out_T_econsistent with output_bot. exists [⊥]. split; try ctx. intuition.
+      - now rewrite <- (vec_map_ext (fun x _ => eval_ident rho x)).
+      - destruct b0. rewrite <-IHphi1, <-IHphi2. now apply Out_T_impl.
+      - destruct q. cbn. setoid_rewrite <-IHphi. setoid_rewrite Out_T_all.
+        setoid_rewrite help. tauto.
+    Qed.
+
+    Definition classical D (I : interp D) :=
+      forall rho phi psi, rho ⊨ (((phi ~> psi) ~> phi) ~> phi).
+
+    Lemma model_bot_classical :
+      classical model_bot.
+    Proof.
+      intros rho phi psi. apply model_bot_correct, Out_T_prv.
+      exists List.nil. split; intuition. apply Pc.
+    Qed.
+
+    Lemma valid_T_model_bot phi :
+      phi ∈ T -> var ⊨ phi.
+    Proof.
+      intros H % (Out_T_sub output_bot). apply model_bot_correct; comp. now rewrite subst_id.
+    Qed.
+
+  End BotModel.
+
+  Section StandardCompletenes.
+    Variables (T : theory) (phi : form).
+    Hypothesis (HT : closed_T T) (Hphi : closed phi).
+
+    Notation "T ⊫S phi" := (forall D (I : interp D) rho, (forall psi, T psi -> rho ⊨ psi) -> rho ⊨ phi) (at level 50).
+
+    Hint Constructors unused.
+
+    Lemma semi_completeness_standard :
+      T ⊫S phi -> ~ ~ T ⊩CE phi.
+    Proof.
+      intros Hval Hcons. rewrite refutation_prv in Hcons. 
+      assert (Hcl : closed_T (T ⋄ (¬ phi))) by ( intros ? ? [] ; subst; eauto).
+      unshelve eapply (model_bot_correct Hcons (¬ phi) var); eauto.
+      - apply Out_T_sub. right. comp. now rewrite subst_id.
+      - apply Hval. intros ? ?. apply valid_T_model_bot; intuition.
+    Qed.
+
+    Lemma completeness_standard_stability :
+      stable (T ⊩CE phi) -> T ⊫S phi -> T ⊩CE phi.
+    Proof.
+      intros Hstab Hsem. now apply Hstab, semi_completeness_standard.
+    Qed.
+  End StandardCompletenes.
+
+  (*Section MPStrongCompleteness.
+    Hypothesis mp : MP.
+    Variable (T : theory) (phi : form).
+    Hypothesis (HT : closed_T T) (Hphi : closed phi).
+    Hypothesis (He : enumerable T).
+
+    Section MPEnum.
+      Variable (X : Type) (P : X -> Prop).
+      Hypothesis (HL : enumerable P) (HX : eq_dec X).
+
+      Lemma enumeration_semi_decidable x :
+        exists (f : nat -> bool), P x <-> tsat f.
+      Proof.
+        destruct HL as [g Hg]. exists (fun n => match g n with Some y => if HX x y then true else false | _ => false end).
+        rewrite (Hg x). split; intros [n Hn].
+        - exists n. rewrite Hn. destruct HX; congruence.
+        - exists n. destruct g; try congruence. destruct HX; congruence.
+      Qed.
+
+      Lemma enumeration_stability x :
+        stable (P x).
+      Proof.
+        intros Hn. destruct (enumeration_semi_decidable x) as [f Hf].
+        apply Hf. apply mp. intros Hf'. apply Hn. intros [m Hm] % Hf. apply Hf'. now exists m.
+      Qed.
+    End MPEnum.
+
+    Lemma mp_tprv_stability {p : peirce} :
+      ~ ~ T ⊩ phi -> T ⊩ phi.
+    Proof.
+      apply (enumeration_stability mp (enum_tprv He) (dec_form HdF HdP)).
+    Qed.
+
+    Lemma mp_standard_completeness :
+      T ⊫S phi -> T ⊩CE phi.
+    Proof.
+      intros Hprv % semi_completeness_standard. 2,3: assumption.
+      now apply mp_tprv_stability.
+    Qed.
+  End MPStrongCompleteness.*)
+
+End Completeness.
+
+(*
+(* *** Exploding Models **)
+
+  Section ExplodingCompletenes.
+    Variables (T : theory) (phi : form).
+    Hypothesis (HT : closed_T T) (Hphi : closed phi).
+
+    Lemma completeness_expl :
+      T ⊫E phi -> T ⊩CE phi.
+    Proof.
+      intros Hval. assert (Hcl : closed_T (T ⋄ (¬ phi))) by (intros ? ? [] ; subst; eauto).
+      apply refutation_prv. apply (@Out_T_econsistent _ _ (output_bot Hcl)); cbn. use_theory [⊥]. 2: ctx.
+      intros ? [<- | []]. apply (model_bot_correct _ ⊥ ids).
+      specialize (Hval term (model_bot Hcl) (model_bot_exploding Hcl) ids).
+      assert (@sat _ _ (model_bot Hcl) ids (¬ phi)) by (apply model_bot_correct, Out_T_sub; comp; firstorder).
+      apply H, Hval. intros ? ?. apply valid_T_model_bot; intuition.
+    Qed.
+
+    Lemma valid_standard_expld_stability :
+      (T ⊫S phi -> T ⊫E phi) <-> stable (T ⊩CE phi).
+    Proof.
+      rewrite <- completeness_standard_stability. 2,3: assumption. split.
+      - intros Hincl Hval % Hincl. now apply completeness_expl.
+      - intros Hcomp Hprv % Hcomp. apply (StrongSoundness Hprv).
+        all: now intros _ ? ? [].
+    Qed.
+  End ExplodingCompletenes.
+
+(* *** Minimal Models **)
+
+  Section FragmentModel.
+    Variable T : theory.
+    Hypothesis T_closed : closed_T T.
+
+    Variable GBot : form.
+    Hypothesis GBot_closed : closed GBot.
+
+    Definition input_fragment :=
+      {|
+        NBot := GBot ;
+        NBot_closed := GBot_closed ;
+
+        variant := lconst ;
+
+        In_T := T ;
+        In_T_closed := T_closed ;
+
+        GenConstructions.enum := form_enum ;
+        enum_enum := form_enum_enumerates ;
+        enum_unused := form_enum_fresh
+      |}.
+
+    Definition output_fragment := construct_construction input_fragment.
+
+    Instance model_fragment : interp term :=
+      {| i_f := Func; i_P := fun P v => Pred P v ∈ Out_T output_fragment ;
+        i_F := ⊥ ∈ Out_T output_fragment |}.
+
+    Lemma eval_ident_fragment rho (t : term) :
+      eval rho t = subst_term rho t.
+    Proof.
+      induction t using strong_term_ind; comp; asimpl; try congruence. f_equal.
+    Qed.
+
+    Lemma model_fragment_correct phi rho :
+      (phi[rho] ∈ Out_T output_fragment <-> rho ⊨ phi).
+    Proof.
+      induction phi in rho |-*. 1,2,3: comp.
+      - tauto.
+      - now rewrite <- (vec_ext (fun x => eval_ident_fragment rho x)).
+      - rewrite <-IHphi1, <-IHphi2. now apply Out_T_impl.
+      - cbn. setoid_rewrite <-IHphi. rewrite Out_T_all.
+        split; intros H d; specialize (H d); comp; now asimpl in H.
+    Qed.
+
+    Lemma model_fragment_classical :
+      BLM model_fragment.
+    Proof.
+      intros rho phi psi. apply model_fragment_correct, Out_T_prv.
+      use_theory (nil : list form). apply Pc.
+    Qed.
+
+    Lemma valid_T_fragment phi :
+      phi ∈ T -> ids ⊨ phi.
+    Proof.
+      intros H % (Out_T_sub output_fragment). apply model_fragment_correct; now comp.
+    Qed.
+  End FragmentModel.
+
+  Section FragmentCompleteness.
+
+    Lemma semi_completeness_fragment T phi :
+      closed_T T -> closed phi -> T ⊫M phi -> T ⊩CL phi.
+    Proof.
+      intros HT Hphi Hval. replace phi with (phi[ids]) in * by now comp.
+      apply (@Out_T_econsistent _ _ (output_fragment HT Hphi)); cbn. use_theory [phi[ids]]. 2: ctx.
+      intros ? [<- | []]. apply (model_fragment_correct HT Hphi phi ids). comp. rewrite instId_form in Hval.
+      apply Hval. 1: apply model_fragment_classical. intros ? ?. apply valid_T_fragment; intuition.
+    Qed.
+  End FragmentCompleteness.
+End Completeness.
+
+(* ** Extending the Completeness Results *)
+
+Section FiniteCompleteness.
+  Context {Sigma : Signature}.
+  Context {HdF : eq_dec Funcs} {HdP : eq_dec Preds}.
+  Context {HeF : enumT Funcs} {HeP : enumT Preds}.
+
+  Lemma list_completeness_standard A phi :
+    ST__f -> valid_L SM A phi -> A ⊢CE phi.
+  Proof.
+    intros stf Hval % valid_L_to_single. apply prv_from_single.
+    apply con_T_correct. apply completeness_standard_stability.
+    1: intros ? ? []. 1: apply close_closed. 2: now apply valid_L_valid_T in Hval.
+    apply stf, fin_T_con_T.
+    - intros ? ? [].
+    - eapply close_closed.
+  Qed.
+
+  Lemma list_completeness_expl A phi :
+    valid_L EM A phi -> A ⊢CE phi.
+  Proof.
+    intros Hval % valid_L_to_single. apply prv_from_single.
+    apply tprv_list_T. apply completeness_expl. 1: intros ? ? [].
+    1: apply close_closed. now apply valid_L_valid_T in Hval.
+  Qed.
+
+  Lemma list_completeness_fragment A phi :
+    valid_L BLM A phi -> A ⊢CL phi.
+  Proof.
+    intros Hval % valid_L_to_single. apply prv_from_single.
+    apply tprv_list_T. apply semi_completeness_fragment. 1: intros ? ? [].
+    1: apply close_closed. now apply valid_L_valid_T in Hval.
+  Qed.
+End FiniteCompleteness.
+
+Section StrongCompleteness.
+  Context {Sigma : Signature}.
+  Context {HdF : eq_dec Funcs} {HdP : eq_dec Preds}.
+  Context {HeF : enumT Funcs} {HeP : enumT Preds}.
+
+  Lemma dn_inherit (P Q : Prop) :
+    (P -> Q) -> ~ ~ P -> ~ ~ Q.
+  Proof. tauto. Qed.
+
+  Lemma strong_completeness_standard (S : stab_class) T phi :
+    (forall (T : theory) (phi : form), S Sigma T -> stable (tmap (fun psi : form => (sig_lift psi)[ext_c]) T ⊩CE phi)) -> @map_closed S Sigma (sig_ext Sigma) (fun phi => (sig_lift phi)[ext_c]) -> S Sigma T -> T ⊫S phi -> T ⊩CE phi.
+  Proof.
+    intros sts cls HT Hval. apply sig_lift_out_T. apply completeness_standard_stability.
+    1: apply lift_ext_c_closes_T. 1: apply lift_ext_c_closes. 2: apply (sig_lift_subst_valid droppable_S Hval).
+    now apply sts.
+  Qed.
+
+  Lemma strong_completeness_expl T phi :
+    T ⊫E phi -> T ⊩CE phi.
+  Proof.
+    intros Hval. apply sig_lift_out_T, completeness_expl.
+    1: apply lift_ext_c_closes_T. 1: apply lift_ext_c_closes.
+    apply (sig_lift_subst_valid droppable_E Hval).
+  Qed.
+
+  Lemma strong_completeness_fragment T phi :
+    T ⊫M phi -> T ⊩CL phi.
+  Proof.
+    intros Hval. apply sig_lift_out_T, semi_completeness_fragment.
+    1: apply lift_ext_c_closes_T. 1: apply lift_ext_c_closes.
+    apply (sig_lift_subst_valid droppable_BL Hval).
+  Qed.
+
+End StrongCompleteness.
+
+Instance enumT_sum {X Y} :
+  enumT X -> enumT Y -> enumT (X + Y).
+Proof.
+  intros H1 H2.
+  exists (fix f n := match n with 0 => []
+                        | S n => f n ++ map inl (L_T X n) ++ map inr (L_T Y n)
+                end).
+  - eauto.
+  - intros [x | y].
+    + destruct (el_T x) as [n Hn].
+      exists (S n). in_app 2. now in_collect x.
+    + destruct (el_T y) as [n Hn].
+      exists (S n). in_app 3. now in_collect y.
+Qed.
+ 
+*)
